impl_check_valid

src/cbor/pulse/raw/everparse/CBOR.Pulse.Raw.EverParse.Format.fst
@@ -1211,3 +1211,18 @@ ensures exists* v' .
 }
 
 #pop-options
+
+inline_for_extraction
+fn impl_holds_on_raw_data_item
+  (f64: squash SZ.fits_u64)
+  (p: Ghost.erased (raw_data_item -> bool))
+  (impl_p: LowParse.Pulse.Recursive.impl_pred_t serialize_raw_data_item_param p)
+  (input: slice byte)
+  (#pm: perm)
+  (#v: Ghost.erased raw_data_item)
+  requires pts_to_serialized serialize_raw_data_item input #pm v
+  returns res: bool
+  ensures pts_to_serialized serialize_raw_data_item input #pm v ** pure (res == holds_on_raw_data_item p v)
+{
+  LowParse.Pulse.Recursive.impl_pred_recursive serialize_raw_data_item_param (jump_leaf ()) (jump_recursive_step_count_leaf f64) (holds_on_raw_data_item_pred p) impl_p input
+}
